theories/test.v
@@ -223,3 +223,59 @@ Proof.
   steps.
 
 Qed.
+
+Fixpoint MkSItems (items : list sitem) : sitems :=
+  match items with
+  | [] =>
+      INil
+  | item :: items =>
+      ICons item (MkSItems items)
+  end.
+
+Definition MkStruct (items : list sitem) : mexpr :=
+  MStruct (MkSItems items).
+
+Fixpoint MkPathRev (xs : list name) : path :=
+  match xs with
+  | [] =>
+      (* Not supposed to happen. *)
+      PathBase "<error in MkPath>"
+  | [x] =>
+      PathBase x
+  | x :: xs =>
+      PathDot (MkPathRev xs) x
+  end.
+
+Definition MkPath (xs : list name) : path :=
+  MkPathRev (rev xs).
+
+Notation EMkPath xs :=
+  (EPath (MkPath xs)).
+
+(*
+  let module A = struct
+    module B = struct
+      let x = 0
+      let y = x + 1
+    end
+    let z = B.y
+  end
+  in A.z
+ *)
+
+Lemma test_struct_access :
+  let e :=
+    ELetModule "A" (
+      MkStruct [
+        IModule "B" $ MkStruct [
+          ILet (Binding1 (PVar "x") (EInt 0));
+          ILet (Binding1 (PVar "y") (EIntAdd (EVar "x") (EInt 1)))
+        ];
+        ILet (Binding1 (PVar "z") (EMkPath ["B"; "y"]))
+      ]
+    ) $
+    EMkPath ["A"; "z"]
+  in
+  let v := VInt (int.repr 1) in
+  reduces e v.
+Proof. reduces. Qed.
